Removes get_state_aux-referencing lemmas from modifies.
Also updates modifies tests to work with get_state_would_return.

test/core/DY.Test.Core.Trace.Modifies.fst
@@ -9,111 +9,143 @@ open FStar.Set
 /// This generally validates that the modifies analysis is working reasonably
 /// automatically on simple programs, even if they make use of a variety of
 /// trace-modifying features.
-let broad_unmodified_test (prin:principal)
-  : traceful state_id
-  = let* new_rand = mk_rand NoUsage (DY.Core.Label.principal_label prin) 32 in
-    let* msg_ts = send_msg new_rand in
-    trigger_event prin "test_event" (Literal (Seq.Base.empty));*
-    let* _ = recv_msg msg_ts in
-    let* new_sid = new_session_id prin in
-    let* _ = set_state prin new_sid new_rand in
-    return new_sid
+val broad_unmodified_test :
+  principal -> traceful state_id
+let broad_unmodified_test prin =
+  let* new_rand = mk_rand NoUsage (DY.Core.Label.principal_label prin) 32 in
+  let* msg_ts = send_msg new_rand in
+  trigger_event prin "test_event" (Literal (Seq.Base.empty));*
+  let* _ = recv_msg msg_ts in
+  let* new_sid = new_session_id prin in
+  let* _ = set_state prin new_sid new_rand in
+  return new_sid
 
-let broad_unmodified_proof (prin:principal) (tr_in:trace)
-  : Lemma
-    (let (new_sid, tr_out) = broad_unmodified_test prin tr_in in
-     forall (sid:state_id). (
-       sid == new_sid \/
-       get_state_aux prin sid tr_in == get_state_aux prin sid tr_out
-     )
+val broad_unmodified_proof :
+  prin:principal -> sid:state_id ->
+  content_opt:option bytes -> tr_in:trace ->
+  Lemma (
+    let (new_sid, tr_out) = broad_unmodified_test prin tr_in in
+    sid == new_sid \/
+    (get_state_would_return prin sid content_opt tr_in ==>
+     get_state_would_return prin sid content_opt tr_out
     )
-  = let (new_sid, tr_out) = broad_unmodified_test prin tr_in in
-    assert(traceful_modifies (broad_unmodified_test prin) tr_in == singleton (prin, new_sid))
+  )
+let broad_unmodified_proof prin sid content_opt tr_in =
+  let (new_sid, tr_out) = broad_unmodified_test prin tr_in in
+  if sid = new_sid then ()
+  else begin
+    introduce get_state_would_return prin sid content_opt tr_in ==>
+              get_state_would_return prin sid content_opt tr_out
+    with _. traceful_get_state_would_return_later prin sid content_opt (broad_unmodified_test prin) tr_in
+  end
 
 /// This test, similar to the previous, validates the modifies analysis, particularly
 /// ensuring that the traceful option bind with *? works as well.
-let optional_unmodified_test (prin:principal)
-  : traceful (option state_id)
-  = let* new_rand = mk_rand NoUsage (DY.Core.Label.principal_label prin) 32 in
-    let* msg_ts = send_msg new_rand in
-    trigger_event prin "test_event" (Literal (Seq.Base.empty));*
-    let*? _ = recv_msg msg_ts in
-    let* new_sid = new_session_id prin in
-    let* _ = get_state prin new_sid in
-    return (Some new_sid)
+val optional_unmodified_test :
+  principal -> traceful (option state_id)
+let optional_unmodified_test prin =
+  let* new_rand = mk_rand NoUsage (DY.Core.Label.principal_label prin) 32 in
+  let* msg_ts = send_msg new_rand in
+  trigger_event prin "test_event" (Literal (Seq.Base.empty));*
+  let*? _ = recv_msg msg_ts in
+  let* new_sid = new_session_id prin in
+  let* _ = get_state prin new_sid in
+  return (Some new_sid)
 
-let optional_unmodified_proof (prin:principal) (tr_in:trace)
-  : Lemma
-    (let (new_sid_opt, tr_out) = optional_unmodified_test prin tr_in in
-     forall (sid:state_id). (
-       (Some sid) == new_sid_opt \/
-       get_state_aux prin sid tr_in == get_state_aux prin sid tr_out
-     )
+val optional_unmodified_proof :
+  prin:principal -> sid:state_id ->
+  content_opt:option bytes -> tr_in:trace ->
+  Lemma (
+    let (new_sid_opt, tr_out) = optional_unmodified_test prin tr_in in
+    (Some sid) == new_sid_opt \/
+    (get_state_would_return prin sid content_opt tr_in ==>
+     get_state_would_return prin sid content_opt tr_out
     )
-  = let (new_sid_opt, tr_out) = optional_unmodified_test prin tr_in in
-    match new_sid_opt with
-    | None -> assert(traceful_modifies (optional_unmodified_test prin) tr_in == empty)
-    | Some new_sid -> assert(traceful_modifies (optional_unmodified_test prin) tr_in `subset` singleton (prin, new_sid))
+  )
+let optional_unmodified_proof prin sid content_opt tr_in =
+  let (new_sid_opt, tr_out) = optional_unmodified_test prin tr_in in
+  if (Some sid) = new_sid_opt then ()
+  else begin
+    introduce get_state_would_return prin sid content_opt tr_in ==>
+              get_state_would_return prin sid content_opt tr_out
+    with _. traceful_get_state_would_return_later prin sid content_opt (optional_unmodified_test prin) tr_in
+  end
 
 /// The following tests ensure that the automation works despite branching, first
 /// within a pure value, and then in the control flow.
 assume val test_branch : bool
 
-let branch_unmodified_test (prin:principal)
-  : traceful (state_id & state_id)
-  = let* new_rand = mk_rand NoUsage (DY.Core.Label.principal_label prin) 32 in
-    let* msg_ts = send_msg new_rand in
-    trigger_event prin "test_event" (Literal (Seq.Base.empty));*
-    let* _ = recv_msg msg_ts in
-    let* new_sid1 = new_session_id prin in
-    let* new_sid2 = new_session_id prin in
-    let modify_sid = if test_branch then new_sid1 else new_sid2 in
-    let* _ = set_state prin modify_sid new_rand in
-    return (new_sid1, new_sid2)
+val branch_unmodified_test :
+  principal -> traceful (state_id & state_id)
+let branch_unmodified_test prin =
+  let* new_rand = mk_rand NoUsage (DY.Core.Label.principal_label prin) 32 in
+  let* msg_ts = send_msg new_rand in
+  trigger_event prin "test_event" (Literal (Seq.Base.empty));*
+  let* _ = recv_msg msg_ts in
+  let* new_sid1 = new_session_id prin in
+  let* new_sid2 = new_session_id prin in
+  let modify_sid = if test_branch then new_sid1 else new_sid2 in
+  let* _ = set_state prin modify_sid new_rand in
+  return (new_sid1, new_sid2)
 
 /// Without this option, the proof automation gets stuck working through
 /// "extraneous" steps.
 #push-options "--z3cliopt 'smt.qi.eager_threshold=100'"
-let branch_unmodified_proof (prin:principal) (tr_in:trace)
-  : Lemma
-    (let ((new_sid1, new_sid2), tr_out) = branch_unmodified_test prin tr_in in
-     forall (sid:state_id). (
-       sid == new_sid1 \/
-       sid == new_sid2 \/
-       get_state_aux prin sid tr_in == get_state_aux prin sid tr_out
-     )
+val branch_unmodified_proof :
+  prin:principal -> sid:state_id ->
+  content_opt:option bytes -> tr_in:trace ->
+  Lemma (
+    let ((new_sid1, new_sid2), tr_out) = branch_unmodified_test prin tr_in in
+    sid == new_sid1 \/
+    sid == new_sid2 \/
+    (get_state_would_return prin sid content_opt tr_in ==>
+     get_state_would_return prin sid content_opt tr_out
     )
-  = let ((new_sid1, new_sid2), tr_out) = branch_unmodified_test prin tr_in in
-    assert(traceful_modifies (branch_unmodified_test prin) tr_in `subset` (as_set [(prin, new_sid1); (prin, new_sid2)]));
-    ()
+  )
+let branch_unmodified_proof prin sid content_opt tr_in =
+  let ((new_sid1, new_sid2), tr_out) = branch_unmodified_test prin tr_in in
+  if sid = new_sid1 || sid = new_sid2 then ()
+  else begin
+    introduce get_state_would_return prin sid content_opt tr_in ==>
+              get_state_would_return prin sid content_opt tr_out
+    with _. traceful_get_state_would_return_later prin sid content_opt (branch_unmodified_test prin) tr_in
+  end
 #pop-options
 
-let branch_unmodified_test_2 (prin:principal)
-  : traceful (state_id & state_id)
-  = let* new_rand = mk_rand NoUsage (DY.Core.Label.principal_label prin) 32 in
-    let* msg_ts = send_msg new_rand in
-    trigger_event prin "test_event" (Literal (Seq.Base.empty));*
-    let* _ = recv_msg msg_ts in
-    let* new_sid1 = new_session_id prin in
-    let* new_sid2 = new_session_id prin in
-    if test_branch
-    then (
-      let* _ = set_state prin new_sid1 new_rand in
-      return (new_sid1, new_sid2)
-    )
-    else
+val branch_unmodified_test_2 :
+  principal -> traceful (state_id & state_id)
+let branch_unmodified_test_2 prin =
+  let* new_rand = mk_rand NoUsage (DY.Core.Label.principal_label prin) 32 in
+  let* msg_ts = send_msg new_rand in
+  trigger_event prin "test_event" (Literal (Seq.Base.empty));*
+  let* _ = recv_msg msg_ts in
+  let* new_sid1 = new_session_id prin in
+  let* new_sid2 = new_session_id prin in
+  if test_branch
+  then (
+    let* _ = set_state prin new_sid1 new_rand in
     return (new_sid1, new_sid2)
+  )
+  else
+  return (new_sid1, new_sid2)
 
 #push-options "--z3cliopt 'smt.qi.eager_threshold=100'"
-let branch_unmodified_proof_2 (prin:principal) (tr_in:trace)
-  : Lemma
-    (let ((new_sid1, new_sid2), tr_out) = branch_unmodified_test_2 prin tr_in in
-     forall (sid:state_id). (
-       sid == new_sid1 \/
-       get_state_aux prin sid tr_in == get_state_aux prin sid tr_out
-     )
+val branch_unmodified_proof_2 :
+  prin:principal -> sid:state_id ->
+  content_opt:option bytes -> tr_in:trace ->
+  Lemma (
+    let ((new_sid1, new_sid2), tr_out) = branch_unmodified_test_2 prin tr_in in
+    sid == new_sid1 \/
+    (get_state_would_return prin sid content_opt tr_in ==>
+     get_state_would_return prin sid content_opt tr_out
     )
-  = let ((new_sid1, new_sid2), tr_out) = branch_unmodified_test_2 prin tr_in in
-    assert(traceful_modifies (branch_unmodified_test_2 prin) tr_in `subset` (singleton (prin, new_sid1)));
-    ()
+  )
+let branch_unmodified_proof_2 prin sid content_opt tr_in =
+  let ((new_sid1, new_sid2), tr_out) = branch_unmodified_test_2 prin tr_in in
+  if sid = new_sid1 then ()
+  else begin
+    introduce get_state_would_return prin sid content_opt tr_in ==>
+              get_state_would_return prin sid content_opt tr_out
+    with _. traceful_get_state_would_return_later prin sid content_opt (branch_unmodified_test_2 prin) tr_in
+  end
  #pop-options
